Taskin/detProds.thy
@@ -7,47 +7,11 @@ text
  \<open>(A,w)\<close>. In this case we could replace every occurrence of \<open>A\<close> with \<open>w\<close> on the right-hand sides of the productions and the 
  language of the grammar would be preserved\<close>
 
-text 
-\<open>\<open>substW xs y ys\<close> replaces every occurrence of the element \<open>y\<close> with the list of elements \<open>ys\<close> in the given list \<open>xs\<close>\<close>
-
-definition "substW y ys xs = concat (map (\<lambda>x. if x=y then ys else [x]) xs)"
-
-lemma substW_simps[simp]:
-  "substW y ys[]  = []"
-  "substW y ys (x#xs) = (if x = y then ys @ substW y ys xs else x # substW y ys xs)"
-unfolding substW_def by auto
-
-subsection \<open>Properties of \<open>substW\<close>\<close>
-
-lemma substW_split: "substW y ys (xs @ xs') = substW y ys xs @ substW y ys xs'"
-unfolding substW_def by auto
-
-lemma substW_skip: "y \<notin> set xs \<Longrightarrow> substW y ys xs = xs"
-unfolding substW_def by (induction xs) auto
-
-lemma substW_len: "length (substW y [y'] xs) = length xs"
-unfolding substW_def by (induction xs) auto
-
-lemma substW_rev: "y' \<notin> set xs \<Longrightarrow> substW y' [y] (substW y [y'] xs) = xs"
-unfolding substW_def by (induction xs) auto
-
-lemma substW_der:
-  "(B,v) \<in> P \<Longrightarrow> P \<turnstile> u \<Rightarrow>* substW (Nt B) v u"
-unfolding substW_def
-proof (induction u)
-  case Nil
-  then show ?case by simp
-next
-  case (Cons a u)
-  then show ?case
-    by (auto simp add: derives_Cons_rule derives_prepend derives_Cons)
-qed
-
 text
 \<open>\<open>substP ps s u\<close> replaces every occurrence of the symbol \<open>s\<close> with the list of symbols \<open>u\<close> on the right-hand sides of the production list \<open>ps\<close>\<close>
 
 definition substP :: "('n, 't) sym \<Rightarrow>  ('n, 't) syms \<Rightarrow> ('n, 't) prods \<Rightarrow> ('n, 't) prods" where
-  "substP s u ps = map (\<lambda>(A,v). (A, substW s u v)) ps"
+  "substP s u ps = map (\<lambda>(A,v). (A, substs s u v)) ps"
 
 subsection \<open>Properties of \<open>substP\<close>\<close>
 
@@ -55,10 +19,10 @@ lemma substP_split: "substP s u (ps @ ps') = substP s u ps @ substP s u ps'"
   by (simp add: substP_def)
 
 lemma substP_skip1: "s \<notin> set v \<Longrightarrow> substP s u ((A,v) # ps) = (A,v) # substP s u ps"
-  by (auto simp add: substW_skip substP_def)
+  by (auto simp add: substs_skip substP_def)
 
 lemma substP_skip2: "s \<notin> syms ps \<Longrightarrow> substP s u ps = ps"
-  by (induction ps) (auto simp add: substP_def substW_skip)
+  by (induction ps) (auto simp add: substP_def substs_skip)
 
 lemma substP_rev: "Nt B \<notin> syms ps \<Longrightarrow> substP (Nt B) [s] (substP s [Nt B] ps) = ps"
 proof (induction ps)
@@ -67,19 +31,19 @@ proof (induction ps)
     by (simp add: substP_def)
 next
   case (Cons a ps)
-  let ?A = "fst a" let ?u = "snd a" let ?substs = "substW s [Nt B]"
+  let ?A = "fst a" let ?u = "snd a" let ?substs = "substs s [Nt B]"
   have "substP (Nt B) [s] (substP s [Nt B] (a # ps)) = substP (Nt B) [s] (map (\<lambda>(A,v). (A, ?substs v)) (a#ps))"
     by (simp add: substP_def)
   also have "... = substP (Nt B) [s] ((?A, ?substs ?u) # map (\<lambda>(A,v). (A, ?substs v)) ps)"
     by (simp add: case_prod_unfold)
-  also have "... = map ((\<lambda>(A,v). (A, substW (Nt B) [s] v))) ((?A, ?substs ?u) # map (\<lambda>(A,v). (A, ?substs v)) ps)"
+  also have "... = map ((\<lambda>(A,v). (A, substsNt B [s] v))) ((?A, ?substs ?u) # map (\<lambda>(A,v). (A, ?substs v)) ps)"
     by (simp add: substP_def)
-  also have "... = (?A, substW (Nt B) [s] (?substs ?u)) # substP (Nt B) [s] (substP s [Nt B] ps)"
+  also have "... = (?A, substsNt B [s] (?substs ?u)) # substP (Nt B) [s] (substP s [Nt B] ps)"
     by (simp add: substP_def)
-  also from Cons have "... = (?A, substW (Nt B) [s] (?substs ?u)) # ps"
+  also from Cons have "... = (?A, substsNt B [s] (?substs ?u)) # ps"
     using set_subset_Cons unfolding Syms_def by auto
   also from Cons.prems have "... = (?A, ?u) # ps"
-    using substW_rev unfolding Syms_def by force
+    using substs_rev unfolding Syms_def by force
   also have "... = a # ps" by simp
   finally show ?case .
 qed
@@ -96,13 +60,13 @@ lemma substP_der:
   "(A,u) \<in> set (substP (Nt B) v ps) \<Longrightarrow> set ((B,v) # ps) \<turnstile> [Nt A] \<Rightarrow>* u"
 proof -
   assume "(A,u) \<in> set (substP (Nt B) v ps)"
-  then have "\<exists>u'. (A,u') \<in> set ps \<and> u = substW (Nt B) v u'" 
+  then have "\<exists>u'. (A,u') \<in> set ps \<and> u = substsNt B v u'" 
     using if_set_map by (smt (verit, del_insts) Pair_inject case_prod_conv old.prod.exhaust substP_def)
-  then obtain u' where u'_def: "(A,u') \<in> set ps \<and> u = substW (Nt B) v u'" by blast
+  then obtain u' where u'_def: "(A,u') \<in> set ps \<and> u = substsNt B v u'" by blast
   then have path1: "set ((B,v) # ps) \<turnstile> [Nt A] \<Rightarrow>* u'"
     by (simp add: derive_singleton r_into_rtranclp)
-  have "set ((B,v) # ps) \<turnstile> u' \<Rightarrow>* substW (Nt B) v u'"
-    using substW_der by (metis list.set_intros(1))
+  have "set ((B,v) # ps) \<turnstile> u' \<Rightarrow>* substsNt B v u'"
+    using substs_der by (metis list.set_intros(1))
   with u'_def have path2: "set ((B,v) # ps) \<turnstile> u' \<Rightarrow>* u" by simp
   from path1 path2 show ?thesis by simp
 qed
@@ -130,7 +94,7 @@ lemma substPW_der:
       and A_B_noteq: "A \<noteq> B"
       and B_notin_dom: "B \<notin> lhss ps"
       and B_notin_v: "Nt B \<notin> set v"
-    shows "set (substP (Nt B) v ps) \<turnstile> [Nt A] \<Rightarrow>* substW (Nt B) v u"
+    shows "set (substP (Nt B) v ps) \<turnstile> [Nt A] \<Rightarrow>* substsNt B v u"
 using assms(1) proof (induction rule: derives_induct)
   case base
   then show ?case using assms(2) by simp
@@ -141,23 +105,23 @@ next
     case True
     then have "v = v'" 
       using B_notin_dom step.hyps unfolding Lhss_def by auto
-    then have "substW (Nt B) v (s @ [Nt B'] @ w) = substW (Nt B) v (s @ v' @ w)" 
-      using step.prems B_notin_v True by (simp add: substW_skip substW_split)
+    then have "substsNt B v (s @ [Nt B'] @ w) = substsNt B v (s @ v' @ w)" 
+      using step.prems B_notin_v True by (simp add: substs_skip substs_split)
     then show ?thesis
       using step.IH by argo
   next
     case False
     then have "(B',v') \<in> set ps"
       using step by auto
-    then have "(B', substW (Nt B) v v') \<in> set (substP (Nt B) v ps)"
+    then have "(B', substsNt B v v') \<in> set (substP (Nt B) v ps)"
       by (metis (no_types, lifting) list.set_map pair_imageI substP_def)
     with rtrancl_into_rtrancl show ?thesis
-      by (smt (verit, ccfv_threshold) False step.IH step.prems derive.simps rtranclp.simps substW_simps substW_split sym.inject(1))
+      by (smt (verit, ccfv_threshold) False step.IH step.prems derive.simps rtranclp.simps substs.simps substs_split sym.inject(1))
   qed
 qed
 
 text
-\<open>With the assumption that the non-terminal \<open>B\<close> is not in the list of symbols \<open>u\<close>, \<open>substW u (Nt B) v\<close> reduces to \<open>u\<close>\<close>
+\<open>With the assumption that the non-terminal \<open>B\<close> is not in the list of symbols \<open>u\<close>, \<open>substs u (Nt B) v\<close> reduces to \<open>u\<close>\<close>
 
 lemma only_if_part: 
   assumes "set ((B,v)#ps) \<turnstile> [Nt A] \<Rightarrow>* u"
@@ -166,7 +130,7 @@ lemma only_if_part:
       and B_notin_v: "Nt B \<notin> set v"
       and B_notin_u: "Nt B \<notin> set u"
     shows "set (substP (Nt B) v ps) \<turnstile> [Nt A] \<Rightarrow>* u"
-  by (metis assms substW_skip substPW_der)
+  by (metis assms substs_skip substPW_der)
 
 text
 \<open>Combining the two implications gives us the desired property of language preservation\<close>
